porting refinement proofs, checkpoint

src/rocq/Semantics/Denotation.v
@@ -180,21 +180,23 @@ Section Denotation.
     | DVALUE_Poison => draw dt
     | _ => DVALUE_Base <$> ret dv
     end.
-    
-  Fixpoint freeze {E} `{DrawE -< E} `{FailureE -< E} `{OOME -< E} `{UBE -< E} (dt:dtyp) (dv : dvalue) : itree E dvalue :=
-    let freeze_fields : list dtyp -> list dvalue -> list dvalue -> itree E (list dvalue) :=
-      fix loop (dts:list dtyp) (dvs:list dvalue) (acc : list dvalue) : itree E (list dvalue) :=
-        match dts, dvs with
-        | [], [] => ret (rev_append acc [])
-        | t::ts, v::vs =>
-            v <- freeze t v ;;
-            loop ts vs (v :: acc)
-        | _, _ => raise "freeze_fields: mismatched field types and values"
-        end
-    in
+
+
+  (*
+  Fixpoint freeze {E} `{DrawE -< E} `{FailureE -< E} `{OOME -< E} `{UBE -< E} (dt:dtyp) (dv:dvalue) : itree E dvalue :=
     match dv with
     | DVALUE_Base v => freeze_base dt v
     | DVALUE_Struct _ fields =>
+        let freeze_fields : list dtyp -> list dvalue -> list dvalue -> itree E (list dvalue) :=
+          fix loop (dts:list dtyp) (dvs:list dvalue) (acc : list dvalue) : itree E (list dvalue) :=
+            match dts, dvs with
+            | [], [] => ret (rev_append acc [])
+            | t::ts, v::vs =>
+                v <- freeze t v ;;
+                loop ts vs (v :: acc)
+            | _, _ => raise "freeze_fields: mismatched field types and values"
+            end
+        in
         match dt with
         | DTYPE_Struct p dts =>
             val <- freeze_fields dts fields [] ;;
@@ -209,7 +211,51 @@ Section Denotation.
         | _ => raise "freeze: type mismatch non-array type"
         end
     end.
-     
+  *)
+
+  Definition freeze {E} `{DrawE -< E} `{FailureE -< E} `{OOME -< E} `{UBE -< E} (dt:dtyp) (dv:dvalue) : itree E dvalue :=
+    let f := fix freeze_h dv : dtyp -> itree E dvalue :=
+        let freeze_fields : list dvalue -> list dtyp -> list dvalue -> itree E (list dvalue) :=
+          fix loop (dvs:list dvalue) (dts:list dtyp)  (acc : list dvalue) : itree E (list dvalue) :=
+            match dts, dvs with
+            | [], [] => ret (rev_append acc [])
+            | t::ts, v::vs =>
+                v <- freeze_h v t ;;
+                loop vs ts (v :: acc)
+            | _, _ => raise "freeze_fields: mismatched field types and values"
+            end
+        in
+      match dv with
+      | DVALUE_Base v => fun dt => freeze_base dt v
+      | DVALUE_Struct _ fields =>
+          fun dt =>
+          match dt with
+          | DTYPE_Struct p dts =>
+              val <- freeze_fields fields dts [] ;;
+              ret (DVALUE_Struct p val)
+          | _ => raise "freeze: type mismatch non-struct type"
+          end
+      | DVALUE_Array _ elts =>
+          fun dt =>
+            match dt with
+            | DTYPE_Array v sz t =>
+                let freeze_elts : list dvalue -> list dvalue -> itree E (list dvalue) :=
+                  fix loop (dvs:list dvalue) (acc:list dvalue) : itree E (list dvalue) :=
+                    match dvs with
+                    | [] => ret (rev_append acc [])
+                    | v::vs =>
+                        v <- freeze_h v t ;;
+                        loop vs (v::acc)
+                    end
+                in
+                val <- freeze_elts elts [];;
+                ret (DVALUE_Array v val)
+            | _ => raise "freeze: type mismatch non-array type"
+            end
+      end
+    in f dv dt.
+
+                       
   Definition NONE := DVALUE_Base (DVALUE_None).
   
   Fixpoint denote_exp (top:option dtyp) (o:exp dtyp) {struct o} : MCFGtop dvalue :=
